Cslib/Logics/Semantics/IPL.lean
@@ -1,0 +1,135 @@
+/-
+Copyright (c) 2025 Thomas Waring. All rights reserved.
+Released under Apache 2.0 license as described in the file LICENSE.
+Authors: Thomas Waring
+-/
+import Cslib.Logics.NaturalDeduction.NJ
+import Mathlib.Order.Heyting.Basic
+import Mathlib.Data.Finset.Fold
+import Mathlib.Order.Fin.Basic
+
+/-! # Heyting-algebra semantics for intuitionistic propositional logic -/
+
+universe u
+
+variable {Atom : Type u} [DecidableEq Atom]
+
+namespace IPL
+
+namespace Semantics
+
+variable {H : Type _} [HeytingAlgebra H]
+
+abbrev Valuation (Atom : Type u) (H : Type _) [HeytingAlgebra H] := Atom → H
+
+variable (v : Valuation Atom H)
+
+open Proposition NJ
+
+/-- The interpretation of a compound formula in a Heyting algebra -/
+def Proposition.interpret : Proposition Atom → H
+  | atom x => v x
+  | bot => ⊥
+  | conj A B => (Proposition.interpret A) ⊓ (Proposition.interpret B)
+  | disj A B => (Proposition.interpret A) ⊔ (Proposition.interpret B)
+  | impl A B => (Proposition.interpret A) ⇨ (Proposition.interpret B)
+
+scoped notation v "[" A "]" => Proposition.interpret v A
+
+-- instance interpPropCoe : CoeFun (Valuation Atom H) (fun _ => Proposition Atom → H) where
+--   coe := Proposition.interpret
+
+def Ctx.interpret (Γ : Ctx Atom) : H := Γ.fold (· ⊓ ·) ⊤ (Proposition.interpret v)
+
+scoped notation v "[" Γ "]" => Ctx.interpret v Γ
+
+-- instance interpCtxCoe : CoeFun (Valuation Atom H) (fun _ => Ctx Atom → H) where
+--   coe := Ctx.interpret
+
+theorem Ctx.interpret_antitone {Γ Δ : Ctx Atom} (h : Γ ⊆ Δ) :
+    v[Δ] ≤ v[Γ] := by
+  have h_disj : Disjoint Γ (Δ \ Γ) := Finset.disjoint_sdiff
+  have hΔ : Γ.disjUnion (Δ \ Γ) h_disj = Δ := by grind
+  have h_top : ⊤ ⊓ ⊤ = (⊤ : H) := top_inf_eq ⊤
+  unfold interpret
+  nth_rw 1 [←h_top]
+  rw [←hΔ, Finset.fold_disjUnion h_disj]
+  exact inf_le_left
+
+
+def Sequent.valid : Sequent Atom → Prop
+  | ⟨Γ,A⟩ => (v[Γ]) ≤ (v[A])
+
+open Derivation
+
+protected theorem sound {S : Sequent Atom} (D : Derivation S) : Sequent.valid v S := by
+  induction D with
+  | ax Γ A =>
+    simp [Sequent.valid, Ctx.interpret]
+  | botE _ _ ih =>
+    dsimp! only at ih ⊢
+    trans ⊥
+    · assumption
+    · exact OrderBot.bot_le _
+  | conjI _ _ ih ih' =>
+    dsimp! only at ih ih' ⊢
+    exact le_inf ih ih'
+  | @conjE₁ _ A B _ ih =>
+    dsimp! only at ih ⊢
+    trans v[A] ⊓ v[B]
+    · assumption
+    · exact inf_le_left
+  | @conjE₂ _ A B _ ih =>
+    dsimp! only at ih ⊢
+    trans v[A] ⊓ v[B]
+    · assumption
+    · exact inf_le_right
+  | @disjI₁ _ A _ _ ih =>
+    dsimp! only at ih ⊢
+    trans v[A]
+    · assumption
+    · exact le_sup_left
+  | @disjI₂ _ _ B _ ih =>
+    dsimp! only at ih ⊢
+    trans v[B]
+    · assumption
+    · exact le_sup_right
+  | @disjE Γ A B C _ _ _ ih₁ ih₂ ih₃ =>
+    dsimp! only at ih₁ ih₂ ih₃ ⊢
+    trans v[insert A Γ] ⊔ v[insert B Γ]
+    · simp only [Ctx.interpret, Finset.fold_insert_idem]
+      rw [←inf_sup_right]
+      apply le_inf
+      · assumption
+      · rfl
+    · apply sup_le <;> assumption
+  | implI Γ _ ih =>
+    dsimp! only at ih ⊢
+    refine le_himp_iff.mpr ?_
+    simpa [Ctx.interpret, inf_comm] using ih
+  | @implE _ A B _ _ ih ih' =>
+    dsimp! only at ih ih' ⊢
+    trans (v[A] ⇨ v[B]) ⊓ v[A]
+    · apply le_inf <;> assumption
+    · exact himp_inf_le
+
+protected theorem sound' {S : Sequent Atom} (h : Derivable S) : Sequent.valid v S :=
+  let ⟨D⟩ := h; IPL.Semantics.sound v D
+
+theorem not_lem_derivable (x : Atom) : ¬ Derivable ⟨∅, (atom x).disj <| impl (atom x) bot⟩ := by
+  intro h
+  let v : Atom → Fin 3 := fun _ => 1
+  have h_sound : _ := IPL.Semantics.sound' v h
+  simp [Sequent.valid, Ctx.interpret, Finset.fold_empty, Top.top, Proposition.interpret,
+    v, Bot.bot, himp] at h_sound
+
+theorem not_dne_derivable (x : Atom) : ¬ Derivable ⟨{impl (atom x) bot |>.impl bot}, atom x⟩ := by
+  intro h
+  let v : Atom → Fin 3 := fun _ => 1
+  have h_sound : _ := IPL.Semantics.sound' v h
+  simp [Sequent.valid, Ctx.interpret, Proposition.interpret, Finset.fold_singleton, v, Top.top,
+    Bot.bot, himp] at h_sound
+
+end Semantics
+
+end IPL
